proof/access-control/ARM/ArchAccess_AC.thy
@@ -23,9 +23,6 @@ lemma arch_troa_tro_alt[Access_AC_assms, elim!]:
    \<Longrightarrow> arch_integrity_obj_alt aag subjects l ko ko'"
   by (fastforce elim: arch_integrity_obj_atomic.cases intro: arch_integrity_obj_alt.intros)
 
-lemma integrity_asids_refl[simp]: "integrity_asids aag subjects ptr s s"
-  by (simp add: integrity_asids_def)
-
 lemma clear_asidpool_trans[elim]:
   "\<lbrakk> asid_pool_integrity subjects aag pool pool';
      asid_pool_integrity subjects aag pool' pool'' \<rbrakk>
@@ -45,43 +42,17 @@ lemma clas_caps_of_state[Access_AC_assms]:
   apply (blast dest: state_asids_to_policy_aux.intros)
   done
 
-lemma trasids_trans:
-  "\<lbrakk> (\<forall>x. integrity_asids aag subjects x (asid_table s (asid_high_bits_of x))
-                                         (asid_table s' (asid_high_bits_of x)));
-     (\<forall>x. integrity_asids aag subjects x (asid_table s' (asid_high_bits_of x))
-                                         (asid_table s'' (asid_high_bits_of x))) \<rbrakk>
-     \<Longrightarrow> (\<forall>x. integrity_asids aag subjects x (asid_table s (asid_high_bits_of x))
-                                             (asid_table s'' (asid_high_bits_of x)))"
-  apply (clarsimp simp: integrity_asids_def)
-  apply metis
-  done
-
 lemma arch_tro_alt_trans_spec[Access_AC_assms]:
   "\<lbrakk> arch_integrity_obj_alt aag subjects l ko ko';
      arch_integrity_obj_alt aag subjects l ko' ko'' \<rbrakk>
      \<Longrightarrow> arch_integrity_obj_alt aag subjects l ko ko''"
   by (fastforce simp: arch_integrity_obj_alt.simps)
 
-lemmas arch_integrity_obj_simps [simp] =
-  trm_orefl[OF refl]
-  trd_orefl[OF refl]
-
-lemma arch_integrity_update_autarch[Access_AC_assms]:
-  "\<lbrakk> arch_integrity_subjects {pasSubject aag} aag (pasMayActivate aag) X st s; is_subject aag ptr \<rbrakk>
-     \<Longrightarrow> arch_integrity_subjects {pasSubject aag} aag (pasMayActivate aag) X st
-                                                  (s\<lparr>kheap := kheap s(ptr \<mapsto> obj)\<rparr>)"
-  unfolding arch_integrity_subjects_def
-  apply (intro conjI,simp_all)
+lemma integrity_asids_update_autarch[Access_AC_assms]:
+  "\<lbrakk> integrity_asids aag subjects x st s; is_subject aag ptr \<rbrakk>
+   \<Longrightarrow> integrity_asids aag subjects x (st :: det_ext state) (s\<lparr>kheap := kheap s(ptr \<mapsto> obj)\<rparr>)"
+  unfolding integrity_asids_def integrity_asids_aux_def
    apply clarsimp
-   apply (drule_tac x = x in spec, erule integrity_mem.cases)
-   apply ((auto intro: integrity_mem.intros)+)[4]
-   apply (erule trm_ipc, simp_all)
-   apply (clarsimp simp: restrict_map_Some_iff tcb_states_of_state_def get_tcb_def)
-  apply clarsimp
-  apply (drule_tac x = x in spec, erule integrity_device.cases)
-    apply (erule integrity_device.trd_lrefl)
-   apply (erule integrity_device.trd_orefl)
-  apply (erule integrity_device.trd_write)
   done
 
 lemma as_user_state_vrefs[Access_AC_assms, wp]:
@@ -106,12 +77,12 @@ qed
 
 context Arch begin global_naming ARM_A
 
-lemma arch_eintegrity_sa_update[Access_AC_assms]:
-  "arch_integrity_subjects subjects aag activate X st (scheduler_action_update f s) =
-   arch_integrity_subjects subjects aag activate X st s"
-  by (simp add: arch_integrity_subjects_def trans_state_update'[symmetric])
+lemma integrity_asids_sa_update[Access_AC_assms]:
+    "integrity_asids aag subjects x (st :: det_ext state) (scheduler_action_update f s) =
+     integrity_asids aag subjects x st s"
+  by (simp add: integrity_asids_def)
 
-lemma auth_ipc_buffers_tro:
+lemma auth_ipc_buffers_tro[Access_AC_assms]:
   "\<lbrakk> integrity_obj_state aag activate subjects s s';
      x \<in> auth_ipc_buffers s' p; pasObjectAbs aag p \<notin> subjects \<rbrakk>
      \<Longrightarrow> x \<in> auth_ipc_buffers s p "
@@ -120,108 +91,18 @@ lemma auth_ipc_buffers_tro:
       fastforce simp: tcb_states_of_state_def get_tcb_def auth_ipc_buffers_def
                split: cap.split_asm arch_cap.split_asm if_split_asm bool.splits)
 
-lemma arch_integrity_trans[Access_AC_assms]:
-  assumes t1: "arch_integrity_subjects subjects aag activate X s s'"
-  and     t2: "arch_integrity_subjects subjects aag activate X s' s''"
-  and   tro1: "integrity_obj_state aag activate subjects s s'"
-  and   tro2: "integrity_obj_state aag activate subjects s' s''"
-  shows       "arch_integrity_subjects subjects aag activate X s s''"
-proof -
-  have intm: "\<forall>x. integrity_mem aag subjects x
-                  (tcb_states_of_state s) (tcb_states_of_state s'') (auth_ipc_buffers s) X
-                  (underlying_memory (machine_state s) x)
-                  (underlying_memory (machine_state s'') x)" (is "\<forall>x. ?P x s s''")
-  proof
-    fix x
-    from t1 t2 have m1: "?P x s s'" and m2: "?P x s' s''"
-      unfolding integrity_subjects_def arch_integrity_subjects_def by auto
+lemma trasids_trans[Access_AC_assms]:
+  "\<lbrakk> (\<forall>x. integrity_asids aag subjects x s s');
+     (\<forall>x. integrity_asids aag subjects x  s' s'')\<rbrakk>
+   \<Longrightarrow>
+     (\<forall>x. integrity_asids aag subjects x s s'')"
+  apply (clarsimp simp: integrity_asids_def integrity_asids_aux_def)
+  apply metis (* FIXME ryanb *)
+  done
 
-    from m1 show "?P x s s''"
-    proof cases
-      case trm_lrefl thus ?thesis by (rule integrity_mem.intros)
-    next
-      case trm_globals thus ?thesis by (rule integrity_mem.intros)
-    next
-      case trm_orefl
-      from m2 show ?thesis
-      proof cases
-        case (trm_ipc p')
-
-        show ?thesis
-        proof (rule integrity_mem.trm_ipc)
-          from trm_ipc show "case_option False can_receive_ipc (tcb_states_of_state s p')"
-            by (fastforce split: option.splits dest: can_receive_ipc_backward [OF tro1])
-
-          from trm_ipc show "x \<in> auth_ipc_buffers s p'"
-            by (fastforce split: option.splits intro: auth_ipc_buffers_tro [OF tro1])
-        qed (simp_all add: trm_ipc)
-      qed (auto simp add: trm_orefl intro: integrity_mem.intros)
-    next
-      case trm_write thus ?thesis by (rule integrity_mem.intros)
-    next
-      case (trm_ipc p')
-      note trm_ipc1 = trm_ipc
-
-      from m2 show ?thesis
-      proof cases
-        case trm_orefl
-        thus ?thesis using trm_ipc1
-          by (auto intro!: integrity_mem.trm_ipc
-                     simp: restrict_map_Some_iff
-                     elim!: tsos_tro_running[OF tro2, rotated])
-      next
-        case (trm_ipc p'')
-        show ?thesis
-        proof (cases "p' = p''")
-          case True thus ?thesis using trm_ipc trm_ipc1 by (simp add: restrict_map_Some_iff)
-        next
-          (* 2 tcbs sharing same IPC buffer, we can appeal to either t1 or t2 *)
-          case False
-          thus ?thesis using trm_ipc1
-            by (auto intro!: integrity_mem.trm_ipc
-                       simp: restrict_map_Some_iff
-                      elim!: tsos_tro_running[OF tro2, rotated])
-        qed
-      qed (auto simp add: trm_ipc intro: integrity_mem.intros)
-    qed
-  qed
-
-  moreover have "\<forall>x. integrity_device aag subjects x
-                  (tcb_states_of_state s) (tcb_states_of_state s'')
-                  (device_state (machine_state s) x)
-                  (device_state (machine_state s'') x)" (is "\<forall>x. ?P x s s''")
-  proof
-    fix x
-    from t1 t2 have m1: "?P x s s'" and m2: "?P x s' s''"
-      unfolding integrity_subjects_def arch_integrity_subjects_def by auto
-
-    from m1 show "?P x s s''"
-    proof cases
-      case trd_lrefl thus ?thesis by (rule integrity_device.intros)
-    next
-      case torel1: trd_orefl
-      from m2 show ?thesis
-      proof cases
-        case (trd_lrefl) thus ?thesis by (rule integrity_device.trd_lrefl)
-      next
-        case trd_orefl thus ?thesis
-          by (simp add:torel1)
-      next
-        case trd_write thus ?thesis by (rule integrity_device.trd_write)
-      qed
-    next
-      case trd_write thus ?thesis by (rule integrity_device.intros)
-    qed
-  qed
-  thus ?thesis using tro_trans[OF tro1 tro2] t1 t2 intm
-    apply (clarsimp simp: integrity_subjects_def arch_integrity_subjects_def)
-    apply (frule(1) trasids_trans[simplified])
-    by blast
-qed
-
-lemma arch_integrity_refl[Access_AC_assms, simp]:
-  "arch_integrity_subjects S aag activate X s s"
-  unfolding arch_integrity_subjects_def
+lemma integrity_asids_refl[Access_AC_assms, simp]:
+    "integrity_asids aag subjects x (s :: det_ext state) s"
+  unfolding integrity_asids_def integrity_asids_aux_def
   by simp
 
 end
@@ -266,42 +147,26 @@ lemma auth_ipc_buffers_member_def:
   unfolding auth_ipc_buffers_def
   by (clarsimp simp: caps_of_state_tcb' split: option.splits cap.splits arch_cap.splits bool.splits)
 
-lemma trm_ipc':
-  "\<lbrakk> pas_refined aag s; valid_objs s; case_option False can_receive_ipc (tcb_states_of_state s p');
-     (tcb_states_of_state s' p') = Some Running; p \<in> auth_ipc_buffers s p' \<rbrakk>
-     \<Longrightarrow> integrity_mem aag subjects p (tcb_states_of_state s) (tcb_states_of_state s')
-                      (auth_ipc_buffers s) X
-                      (underlying_memory (machine_state s) p)
-                      (underlying_memory (machine_state s') p)"
-  apply (cases "pasObjectAbs aag p' \<in> subjects")
-   apply (rule trm_write)
-   apply (clarsimp simp: auth_ipc_buffers_member_def)
-   apply (frule pas_refined_mem[rotated])
-    apply (erule sta_caps, simp)
-     apply (erule(3) ipcframe_subset_page)
-    apply (fastforce simp: cap_auth_conferred_def arch_cap_auth_conferred_def
-                           vspace_cap_rights_to_auth_def is_page_cap_def)
-   apply fastforce
-  by (rule trm_ipc)
+(* FIXME ryanb: only this version needed? *)
+lemma auth_ipc_buffers_member[Access_AC_assms]:
+  "\<lbrakk> x \<in> auth_ipc_buffers s p; valid_objs s \<rbrakk>
+     \<Longrightarrow> \<exists>tcb acap. get_tcb p s = Some tcb
+                  \<and> tcb_ipcframe tcb = (cap.ArchObjectCap acap)
+                  \<and> caps_of_state s (p, tcb_cnode_index 4) = Some (ArchObjectCap acap)
+                  \<and> Write \<in> arch_cap_auth_conferred acap
+                  \<and> x \<in> aobj_ref' acap"
+  by (fastforce simp: auth_ipc_buffers_def caps_of_state_tcb' arch_cap_auth_conferred_def
+                      vspace_cap_rights_to_auth_def ipcframe_subset_page
+               split: option.splits cap.splits arch_cap.splits bool.splits if_splits)
 
-lemma asid_pool_integrity_mono:
+lemma asid_pool_integrity_mono[Access_AC_assms]:
   "\<lbrakk> asid_pool_integrity S aag cont cont' ; S \<subseteq> T \<rbrakk> \<Longrightarrow> asid_pool_integrity T aag cont cont'"
   unfolding asid_pool_integrity_def by fastforce
 
-lemma arch_integrity_mono[Access_AC_assms]:
-  "\<lbrakk> arch_integrity_subjects S aag activate X s s'; S \<subseteq> T; pas_refined aag s; valid_objs s \<rbrakk>
-     \<Longrightarrow> arch_integrity_subjects T aag activate X s s'"
-  apply (simp add: arch_integrity_subjects_def)
-  apply (rule conjI)
-   apply clarsimp
-   apply (drule_tac x=x in spec, erule integrity_mem.cases;
-           blast intro: integrity_mem.intros trm_ipc')
-  apply (rule conjI)
-   apply clarsimp
-   apply (drule_tac x=x in spec, erule integrity_device.cases;
-          blast intro: integrity_device.intros)
-  apply (fastforce simp: integrity_asids_def)
-  done
+lemma integrity_asids_mono[Access_AC_assms]:
+    "\<lbrakk> integrity_asids aag S x s s'; S \<subseteq> T; pas_refined aag s; valid_objs s \<rbrakk>
+       \<Longrightarrow> integrity_asids aag T x s (s' :: det_ext state)"
+  by (fastforce simp: integrity_asids_def integrity_asids_aux_def)
 
 lemma arch_integrity_obj_atomic_mono[Access_AC_assms]:
   "\<lbrakk> arch_integrity_obj_atomic aag S l ao ao'; S \<subseteq> T; pas_refined aag s; valid_objs s \<rbrakk>
